\begin{activity} \label{A:1.2.1}  Evaluate the following infinite limits analytically.  
\ba
\item 
	\begin{enumerate*}[i)] 
	\item $\ds \lim_{x \to 2^+} \frac{1}{x-2} \quad$ 
	\item $\ds \lim_{x \to 2^-} \frac{1}{x-2} \quad$
	\item $\ds \lim_{x \to 2} \frac{1}{x-2}$ 
	\end{enumerate*}
	
\item 
	\begin{enumerate*}[i)] 
	\item $\ds \lim_{x \to 3^+} \frac{x+2}{(x-3)^3} \quad$ 
	\item $\ds \lim_{x \to 3^-} \frac{x+2}{(x-3)^3} \quad$
	\item $\ds \lim_{x \to 3} \frac{x+2}{(x-3)^3}$ 
	\end{enumerate*}
	
\item
	\begin{enumerate*}[i)] 
	\item $\ds \lim_{x \to 4^+} \frac{x-5}{(x-4)^2} \quad$ 
	\item $\ds \lim_{x \to 4^-} \frac{x-5}{(x-4)^2} \quad$
	\item $\ds \lim_{x \to 4} \frac{x-5}{(x-4)^2}$ 
	\end{enumerate*}
\ea
\end{activity}
\begin{smallhint}
\ba
	\item $(x^2 - 1)$ can be factored.
	\item Expand the expression $(2+x)^3$, and then combine like terms in the numerator.
	\item Try multiplying the given function by this fancy form of 1: $\frac{\sqrt{x+1} + 1}{\sqrt{x+1} + 1}$.
\ea
\end{smallhint}
\begin{bighint}
\ba
	\item $(x^2 - 1) = (x+1)(x-1)$.
	\item Expand the expression $(2+x)^3$ using the rule $(a+b)^3 = a^3 + 3a^2b + 3ab^2 + b^3$, and then combine like terms in the numerator.
	\item Try multiplying the given function by this fancy form of 1: $\frac{\sqrt{x+1} + 1}{\sqrt{x+1} + 1}$.  Expand and simplify the numerator, and then see what happens as $x \to 0$.
\ea
\end{bighint}
\begin{activitySolution}
Estimating the values of the limits with tables is straightforward and should suggest the exact values stated below.
\ba
	\item $\ds \lim_{x \to 1} \frac{x^2 - 1}{x-1} = \lim_{x \to 1} \frac{(x+1)(x-1)}{x-1} = \lim_{x \to 1} (x+1) = 2$. 
	\item $\ds \lim_{x \to 0} \frac{(2+x)^3 - 8}{x} = \lim_{x \to 0} \frac{8 + 12x + 6x^2 + x^3 - 8}{x} = \lim_{x \to 0} \frac{12x + 6x^2 + x^3}{x} =  \lim_{x \to 0} (12 + 6x + x^2) = 12$.
	\item $\ds \lim_{x \to 0} \frac{\sqrt{x+1} - 1}{x} = \lim_{x \to 0} \frac{\sqrt{x+1} - 1}{x} \cdot \frac{\sqrt{x+1} + 1}{\sqrt{x+1} + 1} = \lim_{x \to 0} \frac{x+1-1}{x(\sqrt{x+1}+1)} = \lim_{x \to 0} \frac{1}{\sqrt{x+1}+1} = \frac{1}{2}.$
\ea
\end{activitySolution}
\aftera
