\begin{activity} \label{A:2.4.Act9}  
In this problem, we explore how the limit definition of the derivative more formally shows that $\frac{d}{dx}[\sin(x)] = \cos(x)$.   Letting $f(x) = \sin(x)$, note that the limit definition of the derivative tells us that
	$$f'(x) = \lim_{h \to 0} \frac{\sin(x+h) - \sin(x)}{h}.$$
\ba
	\item Recall the trigonometric identity for the sine of a sum of angles $\alpha$ and $\beta$: $\sin(\alpha + \beta) = \sin(\alpha)\cos(\beta) + \cos(\alpha)\sin(\beta)$.  Use this identity and some algebra to show that
	$$f'(x) = \lim_{h \to 0} \frac{\sin(x)(\cos(h)-1) + \cos(x)\sin(h)}{h}.$$
	\item Next, note that as $h$ changes, $x$ remains constant. Explain why it therefore makes sense to say that
	$$f'(x) = \sin(x) \cdot \lim_{h \to 0} \frac{\cos(h) -1 }{h} + \cos(x) \cdot \lim_{h \to 0} \frac{\sin(h)}{h}.$$
	\item Finally, use small values of $h$ to estimate the values of the two limits in (c):
	$$\lim_{h \to 0} \frac{\cos(h) - 1}{h} \ \ \mbox{and} \ \ \lim_{h \to 0} \frac{\sin(h)}{h}.$$
	\item What do your results in (c) thus tell you about $f'(x)$?
	\item By emulating the steps taken above, use the limit definition of the derivative to argue convincingly that $\frac{d}{dx}[\cos(x)] = -\sin(x).$
\ea 

\end{activity}
%\begin{smallhint}
%\ba
%	\item Recall the constant multiple and sum rules.
%	\item $f'(\frac{\pi}{6})$ tells us the slope of the tangent line at $(\frac{\pi}{6},\frac{\pi}{6})$.
%	\item Find both $(\frac{\pi}{2}, g(\frac{\pi}{2}))$ and $g'(\frac{\pi}{2})$.
%	\item $\sin(\frac{\pi}{2})$ is a constant.
%	\item $P'(a)$ tells us the instantaneous rate of change of $P$ with respect to time at the instant $t = a$, and its units are ``units of $P$ per unit of time.''
%\ea
%\end{smallhint}
%\begin{bighint}
%\ba
%	\item Recall the constant multiple and sum rules.
%	\item $f'(a)$ tells us the slope of the tangent line at $(a,f(a))$.
%	\item Find both a point on the tangent line and the slope of the tangent line.
%	\item $\sin(\frac{\pi}{2})$ is a constant.
%	\item $P'(a)$ tells us the instantaneous rate of change of $P$ with respect to time at the instant $t = a$.
%\ea
%\end{bighint}
%\begin{activitySolution}
%\ba
%	\item By the sum and constant multiple rules, $\frac{dh}{dt} = 3(-\sin(t)) - 4(\cos(t)) = -3\sin(t) - 4\cos(t)$.
%	\item The exact slope of the tangent line to $y = f(x) = 2x + \frac{\sin(x)}{2}$ at $x = \frac{\pi}{6}$ is given by $f'(\frac{\pi}{6})$.  So, we first compute $f'(x)$.  Using the sum and constant multiple rules, $f'(x) = 2 + \frac{1}{2}\cos(x)$, and thus $f'(\frac{\pi}{6}) = 2 + \frac{1}{2} \cos(\frac{\pi}{6}) = 2 + \frac{\sqrt{3}}{4}.$
%	\item The tangent line passes through the point $(\frac{\pi}{2}, g(\frac{\pi}{2}))$ with slope $g'(\frac{\pi}{2})$.  We observe first that $g(\frac{\pi}{2}) = (\frac{\pi}{2})^2 + 2\cos(\frac{\pi}{2}) = \frac{\pi^2}{4}$.  Next, we compute the derivative function, $g'(x)$, and find that
%	$$g'(x) = 2x - 2\sin(x).$$
%	Thus, $g(\frac{\pi}{2}) = 2 \cdot \frac{\pi}{2} - 2 \sin(\frac{\pi}{2}) = \pi - 1$.
%	
%	Hence the equation of the tangent line (in point-slope form) is given by 
%	$$y - \frac{\pi^2}{4} = (\pi-1)(x-\frac{\pi}{2}).$$
%	\item Noting that $\sin(\frac{\pi}{2})$ is a constant, we have $p'(z) = 4z^3 + 4^z \ln(4) - 4\sin(z)$.
	
%	\item The value of $P'(2)$ will tell us the instantaneous rate of change of $P$ at the instant two decades have elapsed.  Observe that $P'(t) = 8\cos(t)$, and thus $P'(2) = 8\cos(2) \approx -3.329$ hundred animals per decade.  This tells us that the instantaneous rate of change of $P$ on January 1, 2030 is about $-3329$ animals per decade, which tells us that the animal population is shrinking considerably at this point in time.  We might say that for whatever the population is on January 1, 2030, we expect that population to drop by about 3300 animals over the next ten years, provided the current population trend continues.
%\ea
%\end{activitySolution}
\aftera