\begin{activity} \label{8.3.Act2} If the \emph{series} $\sum a_k$ converges, then an important result necessarily follows regarding the \emph{sequence} $\{a_n\}$. This activity explores this result. 

Assume that the series $\ds \sum_{k=1}^{\infty} a_k$ 
converges and has sum equal to $L$. 

\ba
\item What is the $n$th partial sum $S_n$ of the series $\ds \sum_{k=1}^{\infty} a_k$?

\item What is the $(n-1)$st partial sum $S_{n-1}$ of the series $\ds \sum_{k=1}^{\infty} a_k$?

\item What is the difference between the $n$th partial sum and the $(n-1)$st partial sum of the series $\ds \sum_{k=1}^{\infty} a_k$?

\item Since we are assuming that  $\ds \sum_{k=1}^{\infty} a_k = L$, what does that tell us about $\ds \lim_{n \to \infty} S_n$? Why?  What does that tell us about $\ds \lim_{n \to \infty} S_{n-1}$? Why?



\item Combine the results of the previous two parts of this activity to determine $\ds \lim_{n \to \infty} a_n = \lim_{n \to \infty} (S_n - S_{n-1})$.


\ea

\end{activity}

\begin{smallhint}
\ba
	\item Small hints for each of the prompts above.
\ea
\end{smallhint}
\begin{bighint}
\ba
	\item Big hints for each of the prompts above.
\ea
\end{bighint}
\begin{activitySolution}
\ba
	\item The $n$th partial sum of the series $\ds \sum_{k=1}^{\infty} a_k$ is
\[S_n = \sum_{k=1}^n a_k.\]
    \item The $(n-1)$st partial sum of the series $\ds \sum_{k=1}^{\infty} a_k$ is
\[S_{n-1} = \sum_{k=1}^{n-1} a_k.\]
    \item The difference between $S_n$ and $S_{n-1}$ is
\[\sum_{k=1}^{n} a_k - \sum_{k=1}^{n-1} a_k = a_{n}.\]
    \item Since  $\ds \sum_{k=1}^{\infty} a_k = \lim_{n \to \infty} S_n$ we must have $\lim_{n \to \infty} S_n = L$. Also,
\[\lim_{n \to \infty} S_n = \lim_{n \to \infty} S_{n-1},\]
so $\lim_{n \to \infty} S_{n-1} = L$ as well.
    \item We have
\begin{align*}
\lim_{n \to \infty} a_n &= \lim_{n \to \infty} \left(S_n - S_{n-1}\right) \\
    &= \lim_{n \to \infty} S_n - \lim_{n \to \infty} S_{n-1} \\
    &= L - L \\
    &= 0.
\end{align*}

\ea
\end{activitySolution}
\aftera 