\begin{example} \label{Ex:2.8.Eg3}
Given $\ds y = \frac{\sqrt{x}(x^2 + 1)^3}{\sin(x)}$, use logarithmic differentiation to find $y'$.

\solution As before, we start by taking the natural log of both sides then applying implicit differentiation.
\begin{align*}
y &= \frac{\sqrt{x}(x^2 + 1)^3}{\sin(x)} \\
\ln{y} &= \ln \left( \frac{\sqrt{x}(x^2 + 1)^3}{\sin(x)}  \right) \enskip \text{\small (apply logarithm rule)} \\
\ln (y) &= \ln \left( \sqrt{x}(x^2 + 1)^3 \right) - \ln( \sin(x) ) \\
\ln (y) &= \ln{\sqrt{x}} + \ln(x^2 + 1)^3 - \ln(\sin(x)) \\
\ln (y) &= \frac{1}{2} \ln(x) + 3\ln(x^2 + 1) - \ln(\sin(x)) \\
\frac{d}{dx}\Big(\ln (y)\Big) &= \frac{d}{dx}\Big( \frac{1}{2} \ln(x) + 3\ln(x^2 + 1) - \ln(\sin(x)) \Big) \\
\frac{y'}{y} &= \frac{1}{2} \cdot \frac{1}{x} + 3\cdot\frac{1}{x^2+1}\cdot 2x - \frac{1}{\sin(x)} \cdot \cos(x) \\
\frac{y'}{y} &= \frac{1}{2x} + \frac{6x}{x^2+1} - \cot(x) \\
y' &=y \left( \frac{1}{2x} + \frac{6x}{x^2+1} - \cot(x) \right) \\
y' &= \frac{\sqrt{x}(x^2 + 1)^3}{\sin(x)} \left( \frac{1}{2x} + \frac{6x}{x^2+1} - \cot(x) \right).
\end{align*} 
\end{example}