\begin{example} \label{Ex:3.6.Eg3}
In each of the following, find the differential $dy$.
\begin{center}
1) $y = \sin x$ \qquad\quad 2) $y = e^x(x^2+2)$ \quad\qquad 3) $y = \sqrt{x^2+3x-1}$
\end{center}

\solution
\begin{enumerate}[1)]
\item $y = \sin x$:	\quad As $f(x) = \sin x$, $\fp(x) = \cos x$. Thus $$dy = \cos (x)dx.$$

\item $y = e^x(x^2+2)$:\quad Let $f(x) = e^x(x^2+2)$. We need $\fp(x)$, requiring the Product Rule. 

We have $\fp(x) = e^x(x^2+2) + 2xe^x$, so $$dy = (e^x(x^2+2) + 2xe^x)dx.$$

\item $y = \sqrt{x^2+3x-1}$:\quad	Let $f(x) = \sqrt{x^2+3x-1}$; we need $\fp(x)$, requiring the Chain Rule.

We have $\ds \fp(x) = \frac{1}{2}(x^2+3x-1)^{-\frac12}(2x+3) = \frac{2x+3}{2\sqrt{x^2+3x-1}}.$ Thus 
$$ dy = \frac{(2x+3)dx}{2\sqrt{x^2+3x-1}}.$$
\end{enumerate}
\end{example}