\begin{example} % EXAMPLE
Evaluate $\ds  \sum_{i=1}^6 (2i-1)$. 

\solution 
\begin{align*}
\sum_{i=1}^6 (2i-1) & = \sum_{i=1}^6 2i - \sum_{i=1}^6 1 \\
& = 2\sum_{i=1}^6 i - \sum_{i=1}^6 1 \\
& = 2 \left( \frac{6(6+1)}{2} \right) - 6 \\
& = 42-6 \\
& = 36
\end{align*}
We obtained the same answer without writing out all six terms. When dealing with small sizes of $n$, it may be faster to write the terms out by hand. However, the Properties of Summations are incredibly important when dealing with large sums as we'll soon see.
\end{example}