\begin{example}
Find $f(t)$, given that $f''(t) = \cos t$, $f'(0) = 3$ and $f(0) = 5$.
We start by finding $f'(t)$, which is an antiderivative of $f''(t)$:
\[ \int f''(t)\ dt = \int \cos t\ dt = \sin t + C = f'(t). \]
	
So $f'(t) = \sin t+C$ for the correct value of $C$. We are given that $f'(0) = 3$, so:
\[ f'(0) = 3 \quad \Rightarrow \quad \sin 0+C = 3 \quad \Rightarrow \quad C=3. \]
Using the initial value, we have found $f'(t) = \sin t+ 3.$
		
We now find $f(t)$ by integrating again.

\[ \int f'(t) \ dt = \int (\sin t+3)\ dt = -\cos t + 3t + C. \]
We are given that $f(0) = 5$, so
\begin{align*}
-\cos 0 + 3(0) + C &= 5 \\
-1 + C &= 5\\
C &= 6
\end{align*}
Thus $f(t) = -\cos t + 3t + 6$.
\end{example}