\begin{marginfigure}[4cm] % MARGIN FIGURE
\subfloat[]{\margingraphics{figures/figseries5a}}
\subfloat[]{\margingraphics{figures/figseries5b}}
\caption{Scatter plots relating to the series in Example \ref{eg:7.2.6}.} \label{F:eg:7.2.6}
\end{marginfigure}

\begin{example} \label{eg:7.2.6} % EXAMPLE
Evaluate the given series.\\

\noindent 1. $\ds\sum_{n=1}^\infty \frac{(-1)^{n+1}\big(n^2-n\big)}{n^3}$\qquad 2. $\ds\sum_{n=1}^\infty \frac{1000}{n!}$\qquad 3. $\ds \frac1{16}+\frac1{25}+\frac1{36}+\frac1{49}+\cdots$

\solution
\begin{enumerate}
\item	We start by using algebra to break the series apart:
\begin{align*}
\sum_{n=1}^\infty \frac{(-1)^{n+1}\big(n^2-n\big)}{n^3} &= \sum_{n=1}^\infty\left(\frac{(-1)^{n+1}n^2}{n^3}-\frac{(-1)^{n+1}n}{n^3}\right) \\
						&= \sum_{n=1}^\infty\frac{(-1)^{n+1}}{n}-\sum_{n=1}^\infty\frac{(-1)^{n+1}}{n^2} \\
						&= \ln(2) - \frac{\pi^2}{12}	\approx	-0.1293.
\end{align*}

This is illustrated in Figure \ref{F:eg:7.2.6}(a).

\item		This looks very similar to the series that involves $e$ in Key Idea \ref{idea:famous_series}. Note, however, that the series given in this example starts with $n=1$ and not $n=0$. The first term of the series in the Key Idea is $1/0! = 1$, so we will subtract this from our result below:
\begin{align*}
		\sum_{n=1}^\infty \frac{1000}{n!} &= 1000\cdot\sum_{n=1}^\infty \frac{1}{n!} \\
							&= 1000\cdot (e-1) \approx  1718.28.
\end{align*}
This is illustrated in Figure \ref{F:eg:7.2.6}(b). The graph shows how this particular series converges very rapidly.


\item		The denominators in each term are perfect squares; we are adding $\ds \sum_{n=4}^\infty \frac{1}{n^2}$ (note  we start with $n=4$, not $n=1$). This series will converge. Using the formula from Concept \ref{idea:famous_series}, we have the following:
\begin{align*}
\sum_{n=1}^\infty \frac1{n^2} &= \sum_{n=1}^3 \frac1{n^2} +\sum_{n=4}^\infty \frac1{n^2} \\
\sum_{n=1}^\infty \frac1{n^2} - \sum_{n=1}^3 \frac1{n^2} &=\sum_{n=4}^\infty \frac1{n^2} \\
\frac{\pi^2}{6} - \left(\frac11+\frac14+\frac19\right) &= \sum_{n=4}^\infty \frac1{n^2} \\
\frac{\pi^2}{6} - \frac{49}{36} &= \sum_{n=4}^\infty \frac1{n^2} \\
0.2838&\approx \sum_{n=4}^\infty \frac1{n^2} 
\end{align*}
\end{enumerate}

\end{example}